wand_demo/bst_lemmas.v
@@ -1,0 +1,172 @@
+Require Import VST.floyd.proofauto.
+Require Import VFA.SearchTree.
+Require Import WandDemo.SearchTree_ext.
+Require Import WandDemo.wand_frame.
+Require Import WandDemo.wandQ_frame.
+Require Import WandDemo.bst.
+
+Instance CompSpecs : compspecs. make_compspecs prog. Defined.
+Definition Vprog : varspecs. mk_varspecs prog. Defined.
+Definition t_struct_tree := Tstruct _tree noattr.
+
+Fixpoint tree_rep (t: tree val) (p: val) : mpred :=
+ match t with
+ | E => !!(p=nullval) && emp
+ | T a x v b => !! (Int.min_signed <= Z.of_nat x <= Int.max_signed /\ tc_val (tptr Tvoid) v) &&
+    EX pa:val, EX pb:val,
+    data_at Tsh t_struct_tree (Vint (Int.repr (Z.of_nat x)),(v,(pa,pb))) p *
+    tree_rep a pa * tree_rep b pb
+ end.
+
+Definition treebox_rep (t: tree val) (b: val) :=
+ EX p: val, data_at Tsh (tptr t_struct_tree) p b * tree_rep t p.
+
+(*
+(* TODO: seems not useful *)
+Lemma treebox_rep_spec: forall (t: tree val) (b: val),
+  treebox_rep t b =
+  EX p: val, 
+  match t with
+  | E => !!(p=nullval) && data_at Tsh (tptr t_struct_tree) p b
+  | T l x v r => !! (Int.min_signed <= x <= Int.max_signed /\ tc_val (tptr Tvoid) v) &&
+      data_at Tsh (tptr t_struct_tree) p b *
+      field_at Tsh t_struct_tree [StructField _key] (Vint (Int.repr x)) p *
+      field_at Tsh t_struct_tree [StructField _value] v p *
+      treebox_rep l (field_address t_struct_tree [StructField _left] p) *
+      treebox_rep r (field_address t_struct_tree [StructField _right] p)
+  end.
+Proof.
+  intros.
+  unfold treebox_rep at 1.
+  f_equal.
+  extensionality p.
+  destruct t; simpl.
+  + apply pred_ext; entailer!.
+  + unfold treebox_rep.
+    apply pred_ext; entailer!.
+    - Intros pa pb.
+      Exists pb pa.
+      unfold_data_at 1%nat.
+      rewrite (field_at_data_at _ t_struct_tree [StructField _left]).
+      rewrite (field_at_data_at _ t_struct_tree [StructField _right]).
+      cancel.
+    - Intros pa pb.
+      Exists pb pa.
+      unfold_data_at 3%nat.
+      rewrite (field_at_data_at _ t_struct_tree [StructField _left]).
+      rewrite (field_at_data_at _ t_struct_tree [StructField _right]).
+      cancel.
+Qed.
+
+
+*)
+
+
+Lemma tree_rep_saturate_local:
+   forall t p, tree_rep t p |-- !! is_pointer_or_null p.
+Proof.
+destruct t; simpl; intros.
+entailer!.
+Intros pa pb. entailer!.
+Qed.
+
+Hint Resolve tree_rep_saturate_local: saturate_local.
+
+Lemma tree_rep_valid_pointer:
+  forall t p, tree_rep t p |-- valid_pointer p.
+Proof.
+intros.
+destruct t; simpl; normalize; auto with valid_pointer.
+Qed.
+Hint Resolve tree_rep_valid_pointer: valid_pointer.
+
+Lemma treebox_rep_saturate_local:
+   forall t b, treebox_rep t b |-- !! field_compatible (tptr t_struct_tree) [] b.
+Proof.
+intros.
+unfold treebox_rep.
+Intros p.
+entailer!.
+Qed.
+
+Hint Resolve treebox_rep_saturate_local: saturate_local.
+
+Lemma tree_rep_nullval: forall t,
+  tree_rep t nullval |-- !! (t = E).
+Proof.
+  intros.
+  destruct t; [entailer! |].
+  simpl tree_rep.
+  Intros pa pb. entailer!.
+Qed.
+
+Hint Resolve tree_rep_nullval: saturate_local.
+
+Lemma treebox_rep_leaf: forall x p b (v: val),
+  is_pointer_or_null v ->
+  Int.min_signed <= Z.of_nat x <= Int.max_signed ->
+  data_at Tsh t_struct_tree (Vint (Int.repr (Z.of_nat x)), (v, (nullval, nullval))) p * data_at Tsh (tptr t_struct_tree) p b |-- treebox_rep (T E x v E) b.
+Proof.
+  intros.
+  unfold treebox_rep, tree_rep. Exists p nullval nullval. entailer!.
+Qed.
+
+Lemma bst_left_entail: forall (t1 t1' t2: tree val) k (v p1 p2 p b: val),
+  Int.min_signed <= Z.of_nat k <= Int.max_signed ->
+  is_pointer_or_null v ->
+  data_at Tsh (tptr t_struct_tree) p b *
+  data_at Tsh t_struct_tree (Vint (Int.repr (Z.of_nat k)), (v, (p1, p2))) p *
+  tree_rep t1 p1 * tree_rep t2 p2
+  |-- treebox_rep t1 (field_address t_struct_tree [StructField _left] p) *
+       (treebox_rep t1'
+         (field_address t_struct_tree [StructField _left] p) -*
+        treebox_rep (T t1' k v t2) b).
+Proof.
+  intros.
+  unfold_data_at 2%nat.
+  rewrite (field_at_data_at _ t_struct_tree [StructField _left]).
+  unfold treebox_rep at 1. Exists p1. cancel.
+
+  rewrite <- wand_sepcon_adjoint.
+  clear p1.
+  unfold treebox_rep.
+  Exists p.
+  simpl.
+  Intros p1.
+  Exists p1 p2.
+  entailer!.
+  unfold_data_at 2%nat.
+  rewrite (field_at_data_at _ t_struct_tree [StructField _left]).
+  cancel.
+Qed.
+
+Lemma bst_right_entail: forall (t1 t2 t2': tree val) k (v p1 p2 p b: val),
+  Int.min_signed <= Z.of_nat k <= Int.max_signed ->
+  is_pointer_or_null v ->
+  data_at Tsh (tptr t_struct_tree) p b *
+  data_at Tsh t_struct_tree (Vint (Int.repr (Z.of_nat k)), (v, (p1, p2))) p *
+  tree_rep t1 p1 * tree_rep t2 p2
+  |-- treebox_rep t2 (field_address t_struct_tree [StructField _right] p) *
+       (treebox_rep t2'
+         (field_address t_struct_tree [StructField _right] p) -*
+        treebox_rep (T t1 k v t2') b).
+Proof.
+  intros.
+  unfold_data_at 2%nat.
+  rewrite (field_at_data_at _ t_struct_tree [StructField _right]).
+  unfold treebox_rep at 1. Exists p2. cancel.
+
+  rewrite <- wand_sepcon_adjoint.
+  clear p2.
+  unfold treebox_rep.
+  Exists p.
+  simpl.
+  Intros p2.
+  Exists p1 p2.
+  entailer!.
+  unfold_data_at 2%nat.
+  rewrite (field_at_data_at _ t_struct_tree [StructField _right]).
+  cancel.
+Qed.
+
+
